Rename clocking predicates
Renamed for consistency with the typing predicates:
    clk_var	      -> wc_var
    clk_vars	      -> wc_vars
    clk_clock	      -> wc_clock
    clk_lexp	      -> wc_lexp
    clk_lexps	      -> wc_lexps
    clk_cexp	      -> wc_cexp
    Well_clocked_eq   -> wc_equation
    Well_clocked_env  -> wc_env
    Well_clocked_node -> wc_node
    Well_clocked      -> wc_global

NLustre/Clocking.v
@@ -22,106 +22,98 @@ Module Type CLOCKING
 
   Implicit Type C: clockenv.
 
-  (* TODO: rename all as per NLustre/Typing.
-           clk_var -> wc_var,
-           clk_vars -> wc_vars,
-           clk_clock -> wc_clock,
-           clk_lexp -> wc_lexp,
-           etc. *)
-
-  Inductive clk_var C (x: ident) ck: Prop :=
+  Inductive wc_var C (x: ident) ck: Prop :=
   | Cv:
       PM.find x C = Some ck ->
-      clk_var C x ck.
+      wc_var C x ck.
 
-  Definition clk_vars C (xs: list ident) ck: Prop :=
-    Forall (fun x => clk_var C x ck) xs.
+  Definition wc_vars C (xs: list ident) ck: Prop :=
+    Forall (fun x => wc_var C x ck) xs.
 
-  Inductive clk_clock C: clock -> Prop :=
+  Inductive wc_clock C: clock -> Prop :=
   | CCbase:
-      clk_clock C Cbase
+      wc_clock C Cbase
   | CCon:
       forall ck x b,
-        clk_clock C ck ->
-        clk_var C x ck ->
-        clk_clock C (Con ck x b).
+        wc_clock C ck ->
+        wc_var C x ck ->
+        wc_clock C (Con ck x b).
 
-  Inductive clk_lexp C: lexp -> clock -> Prop :=
+  Inductive wc_lexp C: lexp -> clock -> Prop :=
   | Cconst:
       forall c,
-        clk_lexp C (Econst c) Cbase
+        wc_lexp C (Econst c) Cbase
   | Cvar:
       forall x ck ty,
-        clk_var C x ck ->
-        clk_lexp C (Evar x ty) ck
+        wc_var C x ck ->
+        wc_lexp C (Evar x ty) ck
   | Cwhen:
       forall e x b ck,
-        clk_lexp C e ck ->
-        clk_var C x ck ->
-        clk_lexp C (Ewhen e x b) (Con ck x b)
+        wc_lexp C e ck ->
+        wc_var C x ck ->
+        wc_lexp C (Ewhen e x b) (Con ck x b)
   | Cunop:
       forall op e ck ty,
-        clk_lexp C e ck ->
-        clk_lexp C (Eunop op e ty) ck
+        wc_lexp C e ck ->
+        wc_lexp C (Eunop op e ty) ck
   | Cbinop:
       forall op e1 e2 ck ty,
-        clk_lexp C e1 ck ->
-        clk_lexp C e2 ck ->
-        clk_lexp C (Ebinop op e1 e2 ty) ck.
+        wc_lexp C e1 ck ->
+        wc_lexp C e2 ck ->
+        wc_lexp C (Ebinop op e1 e2 ty) ck.
 
-  Definition clk_lexps C (les: list lexp)(ck: clock): Prop :=
-    Forall (fun le => clk_lexp C le ck) les.
+  Definition wc_lexps C (les: list lexp)(ck: clock): Prop :=
+    Forall (fun le => wc_lexp C le ck) les.
 
-  Inductive clk_cexp C: cexp -> clock -> Prop :=
+  Inductive wc_cexp C: cexp -> clock -> Prop :=
   | Cmerge:
       forall x t f ck,
-        clk_var C x ck ->
-        clk_cexp C t (Con ck x true) ->
-        clk_cexp C f (Con ck x false) ->
-        clk_cexp C (Emerge x t f) ck
+        wc_var C x ck ->
+        wc_cexp C t (Con ck x true) ->
+        wc_cexp C f (Con ck x false) ->
+        wc_cexp C (Emerge x t f) ck
   | Cite:
       forall b t f ck,
-        clk_lexp C b ck ->
-        clk_cexp C t ck ->
-        clk_cexp C f ck ->
-        clk_cexp C (Eite b t f) ck
+        wc_lexp C b ck ->
+        wc_cexp C t ck ->
+        wc_cexp C f ck ->
+        wc_cexp C (Eite b t f) ck
   | Cexp:
       forall e ck,
-        clk_lexp C e ck ->
-        clk_cexp C (Eexp e) ck.
+        wc_lexp C e ck ->
+        wc_cexp C (Eexp e) ck.
 
-  Inductive Well_clocked_eq C: equation -> Prop :=
+  Inductive wc_equation C: equation -> Prop :=
   | CEqDef:
       forall x ck ce,
-        clk_var C x ck ->
-        clk_cexp C ce ck ->
-        Well_clocked_eq C (EqDef x ck ce)
+        wc_var C x ck ->
+        wc_cexp C ce ck ->
+        wc_equation C (EqDef x ck ce)
   | CEqApp:
       forall xs ck f les,
-        clk_vars C xs ck ->
-        clk_lexps C les ck ->
-        Well_clocked_eq C (EqApp xs ck f les)
+        wc_vars C xs ck ->
+        wc_lexps C les ck ->
+        wc_equation C (EqApp xs ck f les)
   | CEqFby:
       forall x ck v0 le,
-        clk_var C x ck ->
-        clk_lexp C le ck ->
-        Well_clocked_eq C (EqFby x ck v0 le).
+        wc_var C x ck ->
+        wc_lexp C le ck ->
+        wc_equation C (EqFby x ck v0 le).
 
-  Definition Well_clocked_env C : Prop :=
-    forall x ck, PM.find x C = Some ck -> clk_clock C ck.
+  Definition wc_env C : Prop :=
+    forall x ck, PM.find x C = Some ck -> wc_clock C ck.
   
-  Inductive Well_clocked_node : node -> Prop :=
+  Inductive wc_node : node -> Prop :=
   | SNode:
       forall f i o v eqs ingt0 outgt0 defd vout nodup good C,
-        Forall (Well_clocked_eq C) eqs ->
-        clk_vars C (map fst i) Cbase ->
-        clk_vars C (map fst o) Cbase ->
-        Well_clocked_env C ->
-        Well_clocked_node (mk_node f i o v eqs
-                                   ingt0 outgt0 defd vout nodup good).
+        Forall (wc_equation C) eqs ->
+        wc_vars C (map fst i) Cbase ->
+        wc_vars C (map fst o) Cbase ->
+        wc_env C ->
+        wc_node (mk_node f i o v eqs ingt0 outgt0 defd vout nodup good).
 
-  Definition Well_clocked G : Prop :=
-    Forall (fun nd=> Well_clocked_node nd) G.
+  Definition wc_global G : Prop :=
+    Forall (fun nd=> wc_node nd) G.
 
   Inductive Has_clock_eq: clock -> equation -> Prop :=
   | HcEqDef: forall x ck ce,
@@ -133,15 +125,15 @@ Module Type CLOCKING
 
   (** ** Basic properties of clocking *)
 
-  Lemma Well_clocked_nil: Well_clocked nil.
+  Lemma wc_global_nil: wc_global nil.
   Proof.
     apply Forall_nil.
   Qed.
 
-  Lemma clk_var_det:
+  Lemma wc_var_det:
     forall C x ck1 ck2,
-      clk_var C x ck1
-      -> clk_var C x ck2
+      wc_var C x ck1
+      -> wc_var C x ck2
       -> ck1 = ck2.
   Proof.
     intros C x ck1 ck2.
@@ -152,41 +144,41 @@ Module Type CLOCKING
     end.
   Qed.
 
-  Lemma Well_clocked_env_var:
+  Lemma wc_env_var:
     forall C x ck,
-      Well_clocked_env C
-      -> clk_var C x ck
-      -> clk_clock C ck.
+      wc_env C
+      -> wc_var C x ck
+      -> wc_clock C ck.
   Proof.
     intros C x ck Hwc Hcv.
-    unfold Well_clocked_env in Hwc.
+    unfold wc_env in Hwc.
     inversion_clear Hcv as [Hfv].
     apply Hwc with (1:=Hfv).
   Qed.
 
-  Lemma Well_clocked_env_vars:
+  Lemma wc_env_vars:
     forall C xs ck,
       0 < length xs 
-      -> Well_clocked_env C
-      -> clk_vars C xs ck
-      -> clk_clock C ck.
+      -> wc_env C
+      -> wc_vars C xs ck
+      -> wc_clock C ck.
   Proof.
     intros C xs ck Hlen Hwc Hcv.
     destruct xs; simpl in *; try now inv Hlen.
     eapply Forall_cons2 in Hcv as (? & _).
-    eapply Well_clocked_env_var; eauto.
+    eapply wc_env_var; eauto.
   Qed.
 
-  Lemma clk_clock_lexp:
+  Lemma wc_clock_lexp:
     forall C le ck,
-      Well_clocked_env C
-      -> clk_lexp C le ck
-      -> clk_clock C ck.
+      wc_env C
+      -> wc_lexp C le ck
+      -> wc_clock C ck.
   Proof.
     induction le as [| |le IH | |] (* using lexp_ind2 *).
     - inversion_clear 2; now constructor.
     - intros ck Hwc; inversion_clear 1 as [|? ? ? Hcv| | |].
-      apply Well_clocked_env_var with (1:=Hwc) (2:=Hcv).
+      apply wc_env_var with (1:=Hwc) (2:=Hcv).
     - intros ck Hwc.
       inversion_clear 1 as [| |? ? ? ck' Hle Hcv | |].
       constructor; [now apply IH with (1:=Hwc) (2:=Hle)|assumption].
@@ -194,11 +186,11 @@ Module Type CLOCKING
     - intros ck Hwc; inversion_clear 1; auto.    
   Qed.
 
-  Lemma clk_clock_cexp:
+  Lemma wc_clock_cexp:
     forall C ce ck,
-      Well_clocked_env C
-      -> clk_cexp C ce ck
-      -> clk_clock C ck.
+      wc_env C
+      -> wc_cexp C ce ck
+      -> wc_clock C ck.
   Proof.
     induction ce as [i ce1 IH1 ce2 IH2| |].
     - intros ck Hwc.
@@ -208,7 +200,7 @@ Module Type CLOCKING
     - intros ck Hwc; inversion_clear 1 as [|? ? ? ? Hl H1 H2|].
       now apply IHce1.
     - intros ck Hwc; inversion_clear 1 as [| |? ? Hck].
-      apply clk_clock_lexp with (1:=Hwc) (2:=Hck).
+      apply wc_clock_lexp with (1:=Hwc) (2:=Hck).
   Qed.
 
   Lemma clock_no_loops:
@@ -220,11 +212,11 @@ Module Type CLOCKING
     apply IH.  
   Qed.
 
-  Lemma clk_clock_sub:
+  Lemma wc_clock_sub:
     forall C ck x b,
-      Well_clocked_env C
-      -> clk_clock C (Con ck x b)
-      -> clk_var C x ck.
+      wc_env C
+      -> wc_clock C (Con ck x b)
+      -> wc_var C x ck.
   Proof.
     intros C ck x b Hwc Hclock.
     inversion_clear Hclock as [|? ? ? Hclock' Hcv'].
